src/DY.Core.Trace.Manipulation.fst
@@ -1,0 +1,176 @@
+module DY.Core.Trace.Manipulation
+
+open DY.Core.Trace.Type
+open DY.Core.Trace.Invariant
+open DY.Core.Bytes.Type
+open DY.Core.Bytes
+open DY.Core.Label.Type
+
+(*** Trace monad ***)
+
+type crypto a = tr_in:trace -> (a & tr_out:trace{tr_in <$ tr_out})
+
+val (let*): #a:Type -> #b:Type -> x:crypto a -> f:(a -> crypto b) -> crypto b
+let (let*) #a #b x f tr0 =
+  let (x', tr1) = x tr0 in
+  let (y, tr2) = f x' tr1 in
+  (y, tr2)
+
+val return: #a:Type -> a -> crypto a
+let return #a x tr =
+  (x, tr)
+
+val get_trace: crypto trace
+let get_trace tr =
+  (tr, tr)
+
+(*** Generic trace manipulation ***)
+
+val add_event: trace_event -> crypto unit
+let add_event e tr =
+  ((), Snoc tr e)
+
+val event_exists_add_event:
+  e:trace_event -> tr:trace ->
+  Lemma
+  (ensures (
+    let ((), tr_out) = add_event e tr in
+    event_exists tr_out e
+  ))
+  [SMTPat (add_event e tr)]
+let event_exists_add_event e tr = ()
+
+val get_time: crypto nat
+let get_time =
+  let* tr = get_trace in
+  return (DY.Core.Trace.Type.length tr)
+
+(*** Sending messages ***)
+
+val send_msg: bytes -> crypto unit
+let send_msg msg =
+  add_event (MsgSent msg)
+
+val send_msg_invariant:
+  pr:protocol_preds ->
+  msg:bytes -> tr:trace ->
+  Lemma
+  (requires
+    is_publishable pr tr msg /\
+    trace_invariant pr tr
+  )
+  (ensures (
+    let ((), tr_out) = send_msg msg tr in
+    trace_invariant pr tr_out
+  ))
+  [SMTPat (send_msg msg tr); SMTPat (trace_invariant pr tr)]
+let send_msg_invariant pr msg tr = ()
+
+(*** Corruption ***)
+
+val corrupt: pre_pre_label -> crypto unit
+let corrupt who =
+  add_event (Corrupt who)
+
+val corrupt_invariant:
+  pr:protocol_preds ->
+  who:pre_pre_label -> tr:trace ->
+  Lemma
+  (requires
+    trace_invariant pr tr
+  )
+  (ensures (
+    let ((), tr_out) = corrupt who tr in
+    trace_invariant pr tr_out
+  ))
+  [SMTPat (corrupt who tr); SMTPat (trace_invariant pr tr)]
+let corrupt_invariant pr msg tr = ()
+
+(*** Random number generation ***)
+
+val mk_rand: lab:label -> len:nat{len <> 0} -> crypto bytes
+let mk_rand lab len =
+  let* time = get_time in
+  add_event RandGen;*
+  return (Rand lab len time)
+
+val mk_rand_trace_invariant:
+  pr:protocol_preds ->
+  lab:label -> len:nat{len <> 0} -> tr:trace ->
+  Lemma
+  (requires trace_invariant pr tr)
+  (ensures (
+    let (b, tr_out) = mk_rand lab len tr in
+    trace_invariant pr tr_out
+  ))
+  [SMTPat (mk_rand lab len tr); SMTPat (trace_invariant pr tr)]
+let mk_rand_trace_invariant pr lab len tr = ()
+
+val mk_rand_bytes_invariant:
+  pr:protocol_preds ->
+  lab:label -> len:nat{len <> 0} -> tr:trace ->
+  Lemma
+  (ensures (
+    let (b, tr_out) = mk_rand lab len tr in
+    bytes_invariant pr tr_out b
+  ))
+  // We need a way for the SMT pattern to know the value of `pr`
+  // This is done using `trace_invariant`, although it is not necessary for the theorem to hold,
+  // It is certainly around in the context
+  [SMTPat (mk_rand lab len tr); SMTPat (trace_invariant pr tr)]
+let mk_rand_bytes_invariant pr lab len tr =
+  ()
+
+(*** State ***)
+
+val set_state: principal -> nat -> bytes -> crypto unit
+let set_state prin session_id content =
+  add_event (SetState prin session_id content)
+
+val max: int -> int -> int
+let max x y =
+  if x < y then y else x
+
+val compute_new_session_id: principal -> trace -> nat
+let rec compute_new_session_id prin tr =
+  match tr with
+  | Nil -> 0
+  | Snoc tr_init evt -> (
+    match evt with
+    | SetState prin' sess_id _ ->
+      if prin = prin' then
+        max (sess_id+1) (compute_new_session_id prin tr_init)
+      else
+        compute_new_session_id prin tr_init
+    | _ -> compute_new_session_id prin tr_init
+  )
+
+// Sanity check
+val compute_new_session_id_correct:
+  prin:principal -> tr:trace ->
+  sess_id:nat -> state_content:bytes ->
+  Lemma
+  (requires event_exists tr (SetState prin sess_id state_content))
+  (ensures sess_id < compute_new_session_id prin tr)
+let rec compute_new_session_id_correct prin tr sess_id state_content =
+  match tr with
+  | Nil -> ()
+  | Snoc tr_init evt -> (
+    if evt = SetState prin sess_id state_content then ()
+    else (
+      compute_new_session_id_correct prin tr_init sess_id state_content
+    )
+  )
+
+val new_session_id: principal -> crypto nat
+let new_session_id prin =
+  let* tr = get_trace in
+  return (compute_new_session_id prin tr)
+
+val new_state: principal -> bytes -> crypto nat
+let new_state prin content =
+  let* sess_id = new_session_id prin in
+  set_state prin sess_id content;*
+  return sess_id
+
+//TODO: invariant preservation
